Working on instances for MReturns... StateTReturns_bind_inv is probably not provable.

src/coq/Utils/MonadReturnsLaws.v
@@ -9,6 +9,8 @@ From ExtLib Require Import
 
 From Vellvm.Utils Require Import MonadExcLaws PropT.
 
+Local Open Scope monad_scope.
+
 Set Primitive Projections.
 
 Section Laws.
@@ -16,8 +18,6 @@ Section Laws.
   Context (M : Type -> Type).
   Context {Monad : Monad M}.
   Context {Eq1 : @Eq1 M}.
-
-  Local Open Scope monad_scope.
 
   Class MonadReturns :=
     { MReturns : forall {A} (x : A) (ma : M A), Prop;
@@ -32,7 +32,10 @@ Section Laws.
         eq1 ma (ret a) -> MReturns a ma;
 
       MReturns_ret_inv : forall {A} (x y : A),
-          MReturns x (ret y) -> x = y
+          MReturns x (ret y) -> x = y;
+
+      MReturns_Proper :> forall {A} (a : A),
+          Proper (eq1 ==> iff) (MReturns a)
     }.
 
 End Laws.
@@ -42,6 +45,209 @@ Arguments MReturns_bind {M _ _ _ _}.
 Arguments MReturns_bind_inv {M _ _ _ _}.
 Arguments MReturns_ret {M _ _ _ _}.
 Arguments MReturns_ret_inv {M _ _ _ _}.
+
+Section EitherT.
+  Import EitherMonad.
+
+  Context {E : Type}.
+  Context {M : Type -> Type}.
+  Context {HM : Monad M}.
+  Context {EQM : @Eq1 M}.
+  Context {EQV : @Eq1Equivalence M HM EQM}.
+  Context {MRET : @MonadReturns M HM EQM}.
+          
+
+  Definition EitherTReturns {A} (a : A) (ma : eitherT E M A) : Prop
+    := MReturns (inr a) (unEitherT ma).
+
+  Lemma EitherTReturns_bind :
+    forall {A B} (a : A) (b : B) (ma : eitherT E M A) (k : A -> eitherT E M B),
+      EitherTReturns a ma -> EitherTReturns b (k a) -> EitherTReturns b (bind ma k).
+  Proof.
+    intros * Ha Hb.
+    eapply MReturns_bind; eauto.
+  Qed.
+
+  Lemma EitherTReturns_bind_inv :
+    forall {A B} (ma : eitherT E M A) (k : A -> eitherT E M B) (b : B),
+      EitherTReturns b (bind ma k) -> exists a : A , EitherTReturns a ma /\ EitherTReturns b (k a).
+  Proof.
+    intros * Hb.
+    unfold EitherTReturns in *.
+    eapply MReturns_bind_inv in Hb as (ea & Ha & Hb).
+    destruct ea; eauto.
+
+    apply MReturns_ret_inv in Hb.
+    inversion Hb.
+  Qed.
+
+  Lemma EitherTReturns_ret :
+    forall {A} (a : A) (ma : eitherT E M A),
+      eq1 ma (ret a) -> EitherTReturns a ma.
+  Proof.
+    intros * Hma.
+    eapply MReturns_ret; eauto.
+  Qed.
+
+  Lemma EitherTReturns_ret_inv :
+    forall {A} (x y : A),
+      EitherTReturns x (ret y) -> x = y.
+  Proof.
+    intros * H.
+    unfold EitherTReturns in H.
+    eapply MReturns_ret_inv; eauto.
+    eapply MReturns_ret_inv in H.
+    inversion H.
+    apply MReturns_ret.
+    reflexivity.
+  Qed.
+
+  #[global] Instance EitherTReturns_Proper : forall {A} (a : A),
+      Proper (eq1 ==> iff) (EitherTReturns a).
+  Proof.
+    intros A a.
+    unfold Proper, respectful.
+    intros x y H.
+    split; intros Hret; unfold EitherTReturns in *.
+    - eapply MReturns_Proper; eauto.
+      symmetry.
+      auto.
+    - eapply MReturns_Proper; eauto.
+  Qed.
+  
+  Instance MonadReturns_EitherT : MonadReturns (eitherT E M)
+    := { MReturns := fun A => EitherTReturns;
+         MReturns_bind := fun A B => EitherTReturns_bind;
+         MReturns_bind_inv := fun A B => EitherTReturns_bind_inv;
+         MReturns_ret := fun A => EitherTReturns_ret;
+         MReturns_ret_inv := fun A => EitherTReturns_ret_inv
+       }.
+
+End EitherT.
+
+Section StateT.
+  From ITree Require Import
+       ITree
+       Basics.Basics
+       Events.StateFacts
+       Events.State.
+
+  Import Monads.
+
+  From Vellvm Require Import Utils.StateMonads.
+
+  Context {S : Type}.
+  Context {M : Type -> Type}.
+  Context {HM : Monad M}.
+  Context {EQM : @Eq1 M}.
+  Context {EQV : @Eq1Equivalence M HM EQM}.
+  Context {MRET : @MonadReturns M HM EQM}.
+          
+
+  Definition StateTReturns {A} (a : A) (ma : stateT S M A) : Prop
+    := forall s, exists s', MReturns (a, s') (runStateT ma s).
+
+  Lemma StateTReturns_bind :
+    forall {A B} (a : A) (b : B) (ma : stateT S M A) (k : A -> stateT S M B),
+      StateTReturns a ma -> StateTReturns b (k a) -> StateTReturns b (bind ma k).
+  Proof.
+    intros * Ha Hb.
+    unfold StateTReturns in *.
+
+    intros s.
+    specialize (Ha s) as (sa & Ha).
+    specialize (Hb sa) as (sb & Hb).
+
+    exists sb.
+
+    unfold runStateT in *.
+
+    apply MReturns_bind_inv in Ha as (a' & Ha' & Ha).
+    destruct a'.
+    apply MReturns_ret_inv in Ha.
+    inversion Ha; subst.
+
+    apply MReturns_bind_inv in Hb as (b' & Hb' & Hb).
+    destruct b'.
+    apply MReturns_ret_inv in Hb.
+    inversion Hb; subst.
+
+    eapply MReturns_bind.
+    cbn.
+    eapply MReturns_bind; cbn; eauto.
+
+    cbn.
+
+    apply MReturns_ret.
+    reflexivity.
+  Qed.
+
+  Lemma StateTReturns_bind_inv :
+    forall {A B} (ma : stateT S M A) (k : A -> stateT S M B) (b : B),
+      StateTReturns b (bind ma k) -> exists a : A , StateTReturns a ma /\ StateTReturns b (k a).
+  Proof.
+    intros * Hb.
+    unfold StateTReturns in *.
+
+    (* Somehow I need to pull out an `S` state value in order to get
+       `a`, which is the result from `ma` that gets passed to `k`. 
+
+       I don't think I can do this. Suppose `S` is `void`... May not
+       be able to get a state value at all because the type is
+       uninhabited, and then `a` would come out of thin air...
+     *)
+    eexists.
+    split.
+    - intros s.
+      specialize (Hb s) as (sb & Hb).
+      unfold runStateT in *.
+      eapply MReturns_bind_inv in Hb as ((sb' & b') & Ha & Hb).
+      eapply MReturns_bind_inv in Ha as ((sa' & a') & Ha' & Hb').
+      exists sa'.
+      eapply MReturns_bind; eauto.
+      cbn in *.
+      apply MReturns_ret.
+      reflexivity.
+
+
+
+
+    destruct ea; eauto.
+
+    apply MReturns_ret_inv in Hb.
+    inversion Hb.
+  Qed.
+
+  Lemma StateTReturns_ret :
+    forall {A} (a : A) (ma : stateT S M A),
+      eq1 ma (ret a) -> StateTReturns a ma.
+  Proof.
+    intros * Hma.
+    eapply MReturns_ret; eauto.
+  Qed.
+
+  Lemma StateTReturns_ret_inv :
+    forall {A} (x y : A),
+      StateTReturns x (ret y) -> x = y.
+  Proof.
+    intros * H.
+    unfold StateTReturns in H.
+    eapply MReturns_ret_inv; eauto.
+    eapply MReturns_ret_inv in H.
+    inversion H.
+    apply MReturns_ret.
+    reflexivity.
+  Qed.
+
+  Instance MonadReturns_StateT : MonadReturns (stateT S M)
+    := { MReturns := fun A => StateTReturns;
+         MReturns_bind := fun A B => StateTReturns_bind;
+         MReturns_bind_inv := fun A B => StateTReturns_bind_inv;
+         MReturns_ret := fun A => StateTReturns_ret;
+         MReturns_ret_inv := fun A => StateTReturns_ret_inv
+       }.
+
+End StateT.
 
 From ITree Require Import
      ITree
